updates

Veritas.Interleave.fst
@@ -372,22 +372,12 @@ let lemma_filter_interleave_commute (#a:eqtype) (f:a -> bool) (s: seq a) (ss: ss
   Lemma (interleave (filter f s) (map (filter f) ss)) = 
   bind_squash () (lemma_as_squash (lemma_filter_interleave_commute_aux f s ss))
 
-let interleaved_idx_seq (#a:eqtype) (ss: sseq a) (ic: interleave_ctor ss):
-  Tot (seq (idx_elem #a (length ss))) = admit()
-
-let lemma_interleaved_idx_seq (#a:eqtype) (ss:sseq a) (ic:interleave_ctor ss):
-  Lemma (requires True)
-        (ensures (interleave (project_seq (interleaved_idx_seq ss ic)) ss)) = admit()
-
 let partition_idx_seq (#a:eqtype) (#n:nat) (s: seq (idx_elem #a n)):
   Tot (ss:sseq a{length ss = n}) = admit()
-  
-let lemma_interleave_idx_correct1 (#a:eqtype) (ss:sseq a) (ic:interleave_ctor ss):
-  Lemma (requires True)
-        (ensures (partition_idx_seq (interleaved_idx_seq ss ic) = ss)) = admit()
 
-let partition_idx_seq_interleave_ctor (#a:eqtype) (#n:nat) (s:seq (idx_elem #a n)):
-  Tot (interleave_ctor (partition_idx_seq s)) = admit()
+let lemma_partition_idx_seq_interleaving (#a:eqtype) (#n:nat) (s: seq (idx_elem #a n)):
+  Lemma (interleave (project_seq s) (partition_idx_seq s)) = admit()
+
 
 let lemma_partition_idx_prefix_comm 
   (#a:eqtype) (#n:nat) (s:seq (idx_elem #a n)) (i:nat{i <= length s}) (id:nat{id < n}):
@@ -398,3 +388,10 @@ let lemma_partition_idx_extend1 (#a:eqtype) (#n:nat) (s: seq (idx_elem #a n){len
   Lemma (index (partition_idx_seq s) (snd (telem s)) = 
          append1 (index (partition_idx_seq (hprefix s)) (snd (telem s)))
                  (fst (telem s))) = admit()
+
+let interleaved_idx_seq (#a:eqtype) (ss: sseq a) (ic: interleave_ctor ss):
+  Tot (seq (idx_elem #a (length ss))) = admit()
+
+let lemma_interleaved_idx_seq_correct (#a:eqtype) (ss: sseq a) (ic: interleave_ctor ss):
+  Lemma (requires True)
+        (ensures (partition_idx_seq (interleaved_idx_seq ss ic) = ss)) = admit()
